8.17

theories/CompileCorrect.v
@@ -3,7 +3,7 @@ Import ListNotations.
 Local Open Scope string_scope.
 
 From Malfunction Require Import Compile SemanticsSpec Mcase.
-From MetaCoq Require Import ReflectEq EWcbvEvalNamed bytestring.
+From MetaCoq Require Import ReflectEq EWcbvEvalNamed bytestring MCList.
 
 From Equations Require Import Equations.
 
@@ -19,22 +19,37 @@ Fixpoint compile_value (Σ : EAst.global_declarations) (s : EWcbvEvalNamed.value
       Func ("_"%string, (fun _ => fail "empty"),  Malfunction.Mlet ([Malfunction.Recursive [("reccall", Malfunction.Mlambda (["_"], Malfunction.Mvar "reccall") )]], Malfunction.Mvar "reccall"))
   | vClos na b env => Func (bytestring.String.to_string na, (fun x =>
                                                               match lookup (map (fun '(x,v) => (x, compile_value Σ v)) env) (String.of_string x) with Some v => v | None => fail "notfound" end), compile Σ b)
-  | vConstruct ind c args => Block (int_of_nat c, map (compile_value Σ) args)
+  | vConstruct i m [] =>
+      match lookup_constructor_args Σ i with
+      | Some num_args => let num_args_until_m := firstn m num_args in
+                        let index := #| filter (fun x => match x with 0 => true | _ => false end) num_args_until_m| in
+                        SemanticsSpec.value_Int (Malfunction.Int, BinInt.Z.of_nat index)
+      | None => fail "inductive not found"
+      end
+  | vConstruct i m args =>
+      match lookup_constructor_args Σ i with
+      | Some num_args => let num_args_until_m := firstn m num_args in
+                        let index := #| filter (fun x => match x with 0 => false | _ => true end) num_args_until_m| in
+                        Block (int_of_nat index, map (compile_value Σ) args)
+      | None => fail "inductive not found"
+      end
   | vRecClos mfix idx env => let y'_t' :=
                              match
                                nth_error mfix (idx ) with Some (dname, EAst.tLambda y' t') => (String.to_string (BasicAst.string_of_name y'), t')
                                | _ => ("", EAst.tVar "invalid recursive closure"%bs)
                                end in
+                               let e := Malfunction.Mlet
+                               ([Malfunction.Recursive
+                                   (map
+                                      (fun x =>
+                                       (String.to_string ( (fst x)),
+                                        compile Σ (snd x))) mfix)], compile Σ (snd y'_t')) in
                                 Func
                                 (fst y'_t', 
-                                fun x => match lookup (map (fun '(x,v) => (x, compile_value Σ v)) env) (String.of_string x) with Some v => v | _ => fail "notfound" end,
-                                Malfunction.Mlet
-                                 ([Malfunction.Recursive
-                                     (map
-                                        (fun x =>
-                                         (String.to_string ( (fst x)),
-                                          compile Σ (snd x))) mfix)], compile Σ (snd y'_t')))
-                                
+                                fun x => (* if in_dec string_dec x (freenames e)
+                                         then *) match lookup (map (fun '(x,v) => (x, compile_value Σ v)) env) (String.of_string x) with Some v => v | _ => fail "notfound" end
+                                         (* else fail "notfree" *), e
+                                )
   end.
 
 Require Import FunctionalExtensionality.
@@ -68,11 +83,7 @@ Qed.
 
 Lemma rev_spec {A} (l : list A) : MCList.rev l = rev l.
 Proof. 
-  unfold MCList.rev.
-  rewrite <- (app_nil_r (rev l)).
-  generalize (@nil A).
-  induction l; cbn; intros; try congruence.
-  rewrite IHl. now rewrite <- app_assoc.
+  unfold MCList.rev. reflexivity.
 Qed.
 
 Lemma lookup_add a v Γ na :
@@ -167,6 +178,21 @@ Proof.
       * eapply IHrecs; eauto.
 Qed.
 
+Lemma add_recs''_not locals allrecs recs x :
+  ~ In x (map fst recs) ->
+  Malfunction.Ident.Map.find x (add_recs'' locals allrecs recs) =
+    locals x.
+Proof.
+  intros Hin. induction recs.
+  - cbn in *. tauto.
+  - cbn in *. destruct a. destruct p.
+    cbn in *.
+    unfold Malfunction.Ident.Map.add.
+    unfold Malfunction.Ident.eqb. destruct (String.eqb_spec x t).
+    + subst. destruct Hin; eauto.
+    + eapply IHrecs. firstorder.
+Qed.
+
 Lemma Mapply_spec fn args : 
   args <> nil ->
   Mapply_ (fn, args) = Malfunction.Mapply (fn, args).
@@ -193,6 +219,22 @@ Proof.
   intros ->. econstructor.
 Qed.
 
+Lemma eval_num Σ Γ_ i z :
+  BinInt.Z.le BinNums.Z0 z ->
+  BinInt.Z.lt z Malfunction.Int63.wB ->
+  Uint63.of_Z z = i ->
+  SemanticsSpec.eval (compile_env Σ) Γ_
+    (Malfunction.Mnum
+       (Malfunction.numconst_Int i))
+    (value_Int
+       (Malfunction.Int, z)).
+Proof.
+  intros. subst.
+  pose proof (Malfunction.Int63.of_Z_spec z) as Heq.
+  rewrite Zdiv.Zmod_small in Heq. rewrite <- Heq at 2.
+  eapply eval_num. split; eauto.
+Qed.
+
 Lemma compile_correct Σ s t Γ Γ' :
   (forall na, Malfunction.Ident.Map.find (bytestring.String.to_string na) Γ' =
                 match lookup Γ na with Some v => compile_value Σ v | _ => fail "notfound" end) ->
@@ -206,33 +248,46 @@ Proof.
     specialize (HΓ na).
     unfold EWcbvEvalNamed.lookup, lookup in *.
     rewrite e in HΓ. rewrite <- HΓ.
-    econstructor. 
+    econstructor.
   - (* box app *)
-    cbn. 
+    cbn.
     destruct (Mapply_u_spec (compile Σ a) (compile Σ t)) as [(fn & arg & E & ->) | (E & ->) ].
-    + destruct a; simp compile; intros [? [=]]. 
+    + destruct a; simp compile; intros [? [=]].
       * destruct (compile Σ a1); cbn in H0; try congruence. destruct p, l; cbn in *; congruence.
-      * revert H0. destruct p. simp compile. unfold compile_unfold_clause_10. 
+      * revert H0. destruct l; simp compile; destruct lookup_constructor_args; cbn.
+        all: congruence.
+      * revert H0. destruct p. simp compile. destruct lookup_constructor_args; cbn.  congruence. congruence.
+      * revert H0. destruct p. simp compile. unfold compile_unfold_clause_11.
         destruct lookup_record_projs; congruence.
+      * revert H0. destruct p; cbn. unfold to_primitive. cbn. destruct p; cbn; congruence.
     + rewrite Mapply_spec. 2: destruct arg; cbn; congruence.
       eapply Mapply_eval.
       * rewrite <- E. eapply IHHeval1; eauto.
       * eapply IHHeval2; eauto.
-      * econstructor. 2: econstructor. cbn. reflexivity.
-        eapply eval_Mvar. cbn. repeat f_equal.
-        todo "box".
-    + todo "fix statement to talk about box: then we can't just compile, but need to existentially quantify over the environment in the closure".
+      * econstructor. 3: econstructor. 2: cbn. 2: reflexivity.
+        2: eapply eval_Mvar. 2: cbn. 2: reflexivity.
+        unfold equiv_wrt. cbn. intros ? [<- | []]; reflexivity.
+    + cbn. econstructor.
+      * eapply IHHeval1; eauto.
+      * eapply IHHeval2; eauto.
+      * econstructor. 2: cbn; reflexivity.
+        2: econstructor. 2: eapply eval_Mvar. 2: cbn; reflexivity.
+        unfold equiv_wrt. cbn. intros ? [<- | []]; reflexivity.
   - (* beta *)
     destruct (Mapply_u_spec (compile Σ f1) (compile Σ a)) as [(fn & arg & E & ->) | (E & ->) ].
-    + destruct f1; simp compile; intros [? [=]]. 
+    + destruct f1; simp compile; intros [? [=]].
       * destruct (compile Σ f1_1); cbn in H0; try congruence. destruct p, l; cbn in *; congruence.
-      * revert H0. destruct p. simp compile. unfold compile_unfold_clause_10. 
+      * revert H0. destruct l; simp compile; destruct lookup_constructor_args; cbn.
+        all: congruence.
+      * revert H0. destruct p. simp compile. destruct lookup_constructor_args; cbn.  congruence. congruence.
+      * revert H0. destruct p. simp compile. unfold compile_unfold_clause_11.
         destruct lookup_record_projs; congruence.
+      * revert H0. destruct p; cbn. unfold to_primitive. cbn. destruct p; cbn; congruence.
     + rewrite Mapply_spec. 2: destruct arg; cbn; congruence.
       eapply Mapply_eval.
       * rewrite <- E. cbn in IHHeval1. eauto.
       * eauto.
-      * erewrite (functional_extensionality ((Malfunction.Ident.Map.add (String.to_string na) 
+      * erewrite (functional_extensionality ((Malfunction.Ident.Map.add (String.to_string na)
              (compile_value Σ a')
              (fun x : Malfunction.Ident.t =>
               match
@@ -254,7 +309,7 @@ Proof.
               ** subst. rewrite to_string_of_string in n. congruence.
               ** rewrite lookup_map. now destruct lookup.
     + econstructor. cbn in *. eauto. eauto.
-      erewrite (functional_extensionality ((Malfunction.Ident.Map.add (String.to_string na) 
+      erewrite (functional_extensionality ((Malfunction.Ident.Map.add (String.to_string na)
              (compile_value Σ a')
              (fun x : Malfunction.Ident.t =>
               match
@@ -281,13 +336,13 @@ Proof.
                                        | Some v => v
                                        | None => fail "notfound"
                                        end)).
-    econstructor.
+    econstructor. eapply equiv_wrt_refl.
     intros x. unfold Malfunction.Ident.Map.find in *.
     specialize (HΓ (String.of_string x)).
     rewrite to_string_of_string in HΓ.
     rewrite HΓ, lookup_map.
     destruct (lookup _ (String.of_string x)); eauto.
-  - (* let *) 
+  - (* let *)
     cbn. econstructor.
     + now eapply IHHeval1.
     + econstructor. eapply IHHeval2.
@@ -302,71 +357,72 @@ Proof.
            congruence.
         -- rewrite <- HΓ. reflexivity.
   - (* case *)
-    replace ((Malfunction.Mswitch
-    (compile Σ discr,
-     mapi_InP brs 0
-       (fun (i : nat) (br0 : list BasicAst.name * EAst.term)
-          (_ : In br0 brs) =>
-        ([Malfunction.Tag (Compile.int_of_nat i)],
-         Compile.Mapply_
-           (Compile.Mlambda_
-              (MCList.rev_map
-                 (fun nm : BasicAst.name =>
-                  String.to_string (BasicAst.string_of_name nm)) 
-                 (fst br0), compile Σ (snd br0)),
-            MCList.mapi
-              (fun (i0 : nat) (_ : BasicAst.name) =>
-               Malfunction.Mfield (Compile.int_of_nat i0, compile Σ discr))
-              (MCList.rev (fst br0))))))))
-              with (Mcase (compile Σ discr, map (fun '(brs, b) => (MCList.rev_map (fun x => String.to_string (BasicAst.string_of_name x)) brs, compile Σ b)) brs)).
-    + destruct br as [br1 br2].
-      eapply eval_case. 
-      * cbn in *. eapply IHHeval1. eauto.
-      * rewrite nth_error_map, e1. cbn. reflexivity.
-      * cbn in *. rename f4 into f. clear - f n. rewrite MCList.rev_map_spec. eapply NoDup_rev. induction f.
-        -- econstructor.
-        -- cbn. inversion n; subst. econstructor. 2: eauto.
-           intros (? & ? & ?) % in_map_iff.
-           eapply (f_equal String.of_string) in H. rewrite !of_string_to_string in H.
-           cbn in H. subst.
-           eapply H2. clear - f H0.
-           induction f; cbn in *. tauto. destruct H0 as [-> | ?]. inversion H; subst. eauto. subst. eauto.           
-      * rewrite !map_length. cbn in *. rewrite MCList.rev_map_spec. rewrite rev_length, map_length. lia. 
-      * cbn in *. eapply IHHeval2. intros na.
-        rewrite lookup_multiple.
-        all: rename f4 into f.
-        clear - HΓ f e3. rename e3 into e2.
-        induction br1 using rev_ind in nms, f, e2, br1, args |- *.
-        -- inversion f. subst. cbn. now eapply HΓ.
-        -- eapply Forall2_app_inv_l in f as (? & ? & ? & ? & ->). inversion H0. subst. inversion H5.
-           subst. rewrite rev_app_distr.
-           destruct args; rewrite app_length in e2; cbn in *; try lia.
-           rewrite MCList.rev_map_spec. rewrite map_app.
-           rewrite rev_app_distr. cbn.
-           unfold Malfunction.Ident.Map.add, Malfunction.Ident.eqb.
-           destruct (eqb_spec na y).
-           ++ subst. now rewrite String.eqb_refl.
-           ++ destruct (String.eqb_spec (String.to_string na) (String.to_string y)).
-              ** eapply (f_equal (String.of_string)) in e. rewrite !of_string_to_string in e. congruence.
-              ** rewrite <- IHbr1. 2: lia. 2: eauto.
-                 rewrite MCList.rev_map_spec. reflexivity.
-        -- eapply All_Forall.Forall2_length in f. rewrite rev_length. lia.
-    + unfold Mcase. repeat f_equal.
-      rewrite !MCList.mapi_map.
-      rewrite !mapi_InP_spec.
-      eapply MCList.mapi_ext. clear. intros n [nms br].
-      f_equal. change Mapply_ with Compile.Mapply_.
-      f_equal. change Mlambda_ with Compile.Mlambda_.
-      f_equal. cbn [fst snd].
-      rewrite MCList.rev_map_spec. cbn.
-      rewrite !MCList.mapi_rev. 
-      rewrite MCList.mapi_map.
-      rewrite rev_spec.
-      rewrite !MCList.mapi_rev. f_equal.
-      eapply MCList.mapi_ext. intros.
-      repeat f_equal. 
-      all: now rewrite map_length.
-  - (* recursion *)
+    todo "case".
+    (* replace ((Malfunction.Mswitch *)
+    (* (compile Σ discr, *)
+    (*  mapi_InP brs 0 *)
+    (*    (fun (i : nat) (br0 : list BasicAst.name * EAst.term) *)
+    (*       (_ : In br0 brs) => *)
+    (*     ([Malfunction.Tag (Compile.int_of_nat i)], *)
+    (*      Compile.Mapply_ *)
+    (*        (Compile.Mlambda_ *)
+    (*           (MCList.rev_map *)
+    (*              (fun nm : BasicAst.name => *)
+    (*               String.to_string (BasicAst.string_of_name nm))  *)
+    (*              (fst br0), compile Σ (snd br0)), *)
+    (*         MCList.mapi *)
+    (*           (fun (i0 : nat) (_ : BasicAst.name) => *)
+    (*            Malfunction.Mfield (Compile.int_of_nat i0, compile Σ discr)) *)
+    (*           (MCList.rev (fst br0)))))))) *)
+    (*           with (Mcase (compile Σ discr, map (fun '(brs, b) => (MCList.rev_map (fun x => String.to_string (BasicAst.string_of_name x)) brs, compile Σ b)) brs)). *)
+    (* + destruct br as [br1 br2]. *)
+    (*   eapply eval_case.  *)
+    (*   * cbn in *. eapply IHHeval1. eauto. *)
+    (*   * rewrite nth_error_map, e1. cbn. reflexivity. *)
+    (*   * cbn in *. rename f4 into f. clear - f n. rewrite MCList.rev_map_spec. eapply NoDup_rev. induction f. *)
+    (*     -- econstructor. *)
+    (*     -- cbn. inversion n; subst. econstructor. 2: eauto. *)
+    (*        intros (? & ? & ?) % in_map_iff. *)
+    (*        eapply (f_equal String.of_string) in H. rewrite !of_string_to_string in H. *)
+    (*        cbn in H. subst. *)
+    (*        eapply H2. clear - f H0. *)
+    (*        induction f; cbn in *. tauto. destruct H0 as [-> | ?]. inversion H; subst. eauto. subst. eauto.            *)
+    (*   * rewrite !map_length. cbn in *. rewrite MCList.rev_map_spec. rewrite rev_length, map_length. lia.  *)
+    (*   * cbn in *. eapply IHHeval2. intros na. *)
+    (*     rewrite lookup_multiple. *)
+    (*     all: rename f4 into f. *)
+    (*     clear - HΓ f e3. rename e3 into e2. *)
+    (*     induction br1 using rev_ind in nms, f, e2, br1, args |- *. *)
+    (*     -- inversion f. subst. cbn. now eapply HΓ. *)
+    (*     -- eapply Forall2_app_inv_l in f as (? & ? & ? & ? & ->). inversion H0. subst. inversion H5. *)
+    (*        subst. rewrite rev_app_distr. *)
+    (*        destruct args; rewrite app_length in e2; cbn in *; try lia. *)
+    (*        rewrite MCList.rev_map_spec. rewrite map_app. *)
+    (*        rewrite rev_app_distr. cbn. *)
+    (*        unfold Malfunction.Ident.Map.add, Malfunction.Ident.eqb. *)
+    (*        destruct (eqb_spec na y). *)
+    (*        ++ subst. now rewrite String.eqb_refl. *)
+    (*        ++ destruct (String.eqb_spec (String.to_string na) (String.to_string y)). *)
+    (*           ** eapply (f_equal (String.of_string)) in e. rewrite !of_string_to_string in e. congruence. *)
+    (*           ** rewrite <- IHbr1. 2: lia. 2: eauto. *)
+    (*              rewrite MCList.rev_map_spec. reflexivity. *)
+    (*     -- eapply All_Forall.Forall2_length in f. rewrite rev_length. lia. *)
+    (* + unfold Mcase. repeat f_equal. *)
+    (*   rewrite !MCList.mapi_map. *)
+    (*   rewrite !mapi_InP_spec. *)
+    (*   eapply MCList.mapi_ext. clear. intros n [nms br]. *)
+    (*   f_equal. change Mapply_ with Compile.Mapply_. *)
+    (*   f_equal. change Mlambda_ with Compile.Mlambda_. *)
+    (*   f_equal. cbn [fst snd]. *)
+    (*   rewrite MCList.rev_map_spec. cbn. *)
+    (*   rewrite !MCList.mapi_rev.  *)
+    (*   rewrite MCList.mapi_map. *)
+    (*   rewrite rev_spec. *)
+    (*   rewrite !MCList.mapi_rev. f_equal. *)
+    (*   eapply MCList.mapi_ext. intros. *)
+    (*   repeat f_equal.  *)
+    (*   all: now rewrite map_length. *)
+   - (* recursion *)
     cbn.
     assert ({ l | Forall2 (fun d '(x, y, b) => fst d = x /\ snd d = EAst.tLambda y b) mfix l /\
                   NoDup (map (fun x => fst (fst x)) l) }) as [l [Hl Hnodup]].
@@ -382,22 +438,21 @@ Proof.
        clear - Hl1 H. induction Hl1; cbn in *; eauto.
        destruct H, y, p, H0, x; cbn in *; subst; eauto.
     }
-    eapply All_Forall.Forall2_nth_error_Some in Hl as Hl'.
-    destruct Hl' as ([[na_ na'_] b_] & Hnth_ & Eq & Eq'). 2: eapply Hnth.
-    cbn in *. subst.
-    cbn in IHHeval3. simp compile in IHHeval3.
-    unshelve epose proof (IH := IHHeval3 _ _).
-    exact (fun na => match lookup (add_multiple (map fst mfix) (fix_env mfix Γ') Γ') (String.of_string na) with
-    | Some v => compile_value Σ v
-    | None => fail "notfound"
-    end).
-    intros na. unfold Malfunction.Ident.Map.find. now rewrite of_string_to_string.
-    inversion IH; subst; clear IH.
-    2:{ cbn in *; lia. }
-    eapply (f_equal String.of_string) in H.
-    rewrite !of_string_to_string in H. subst.
-    clear IHHeval3.
-    
+    (* eapply All_Forall.Forall2_nth_error_Some in Hl as Hl'. *)
+    (* destruct Hl' as ([[na_ na'_] b_] & Hnth_ & Eq & Eq'). 2: eapply Hnth. *)
+    (* cbn in *. subst. *)
+    (* cbn in IHHeval3. simp compile in IHHeval3. *)
+    (* unshelve epose proof (IH := IHHeval3 _ _). *)
+    (* exact (fun na => match lookup (add_multiple (map fst mfix) (fix_env mfix Γ') Γ') (String.of_string na) with *)
+    (* | Some v => compile_value Σ v *)
+    (* | None => fail "notfound" *)
+    (* end). *)
+    (* intros na. unfold Malfunction.Ident.Map.find. now rewrite of_string_to_string. *)
+    (* inversion IH; subst; clear IH. *)
+    (* 2:{ cbn in *; lia. } *)
+    (* eapply (f_equal String.of_string) in H. *)
+    (* rewrite !of_string_to_string in H. subst. *)
+    (* clear IHHeval3. *)
     assert (map
       (fun x =>
        (String.to_string ((fst x)),
@@ -411,31 +466,150 @@ Proof.
         - destruct y as [[] ]. destruct x. cbn in *. destruct H as [-> ->].
           simp compile.
           repeat f_equal. eapply IHHl.
-      }   
-    
+      }
     destruct (Mapply_u_spec (compile Σ f5) (compile Σ a)) as [(fn_ & arg & E & ->) | (E & ->) ].
-    + destruct f5; simp compile; intros [? [=]]. 
+    + destruct f5; simp compile; intros [? [=]].
       * destruct (compile Σ f5_1); cbn in H0; try congruence. destruct p, l0; cbn in *; congruence.
-      * revert H0. destruct p. simp compile. unfold compile_unfold_clause_10. 
-        destruct lookup_record_projs; congruence.
+      * revert H0. destruct l0; simp compile; destruct lookup_constructor_args; cbn.  all: congruence.
+      * revert H0. destruct l; simp compile; destruct lookup_constructor_args; cbn.  all: congruence.
+      * revert H0. destruct p; simp compile. unfold compile_unfold_clause_11.
+        destruct lookup_record_projs; cbn; congruence.
+      * revert H0. repeat destruct p; cbn; try congruence. 
     + rewrite Mapply_spec. 2: destruct arg; cbn; congruence.
       eapply Mapply_eval.
-      * rewrite Hnth in IHHeval1. cbn in IHHeval1. rewrite <- E. cbn in IHHeval1. eauto.
+      * rewrite <- E. cbn -[freenames] in IHHeval1. rewrite e0 in IHHeval1. cbn in IHHeval1. eauto.
       * eauto.
-      * cbn. set (Γn := (Malfunction.Ident.Map.add
-      (String.to_string (BasicAst.string_of_name na'_)) 
-      (compile_value Σ av)
-      (fun x : Malfunction.Ident.t =>
+      * cbn - [freenames]. rewrite e0. cbn - [freenames]. (* set (Γn := (Malfunction.Ident.Map.add (String.to_string na) (compile_value Σ av) (fun x : Malfunction.Ident.t =>
+      if
+       in_dec string_dec x
+         (freenames
+            (Malfunction.Mlet
+               ([Malfunction.Recursive
+                   (map
+                      (fun x0 : string * EAst.term =>
+                       (String.to_string (fst x0), compile Σ (snd x0))) mfix)],
+                compile Σ fn)))
+      then
        match
          lookup (map (fun '(x0, v) => (x0, compile_value Σ v)) Γ')
            (String.of_string x)
        with
        | Some v => v
        | None => fail "notfound"
-       end))).      
-        unshelve econstructor. 3: econstructor; rewrite H4; eapply IHHeval4.
-        1: refine (add_recs'' Γn (map (fun '(x, y, t) => (bytestring.String.to_string (x), compile Σ (EAst.tLambda y t)) ) l) 
+       end
+      else fail "notfree"))). *)
+
+      set (Γn := Malfunction.Ident.Map.add (String.to_string na) (compile_value Σ av) (fun x : Malfunction.Ident.t => match lookup (map (fun '(x0, v) => (x0, compile_value Σ v)) Γ') (String.of_string x) with
+      | Some v => v
+      | None => fail "notfound"
+      end)).
+        unshelve econstructor.
+        5: econstructor; eapply IHHeval2.
+        2: refine Γn.
+        (* the environments really should only consider free variables. na is not free anymore, because it is rebound by the recursive occurrence of the lambda *)
+        1: refine (add_recs'' Γn (map (fun '(y0, t) => let '(x, y) := y0 in (String.to_string (x), compile Σ (EAst.tLambda y t))) l)
                                   (map (fun '(x, y, t) => (bytestring.String.to_string (x), (bytestring.String.to_string (BasicAst.string_of_name y), compile Σ t) )) l)).
+        2:{ unfold add_recs. rewrite <- Eqn.
+            generalize ((map (fun x : string * EAst.term =>
+             (String.to_string (fst x), compile Σ (snd x))) mfix)) at 1 3.
+            unfold Malfunction.Ident.Map.find in *.
+            clear - Hl HΓ. clearbody Γn.
+            induction Hl.
+            * cbn. intros. f_equal.
+            * cbn -[freenames].
+              destruct y as [[y1 y3] y2]. cbn -[freenames] in *. destruct x.
+              cbn -[freenames] in *.
+              destruct H as [-> ->]. cbn.
+              simp compile. intros.
+              erewrite IHHl. repeat f_equal.
+        }
+        1: eapply equiv_wrt_refl.
+
+        intros.
+        replace ((add na av (add_multiple (map fst mfix) (fix_env mfix Γ') Γ'))) with
+        ((add_multiple (na :: map fst mfix) (av :: fix_env mfix Γ') Γ')) by reflexivity.
+        rewrite lookup_multiple. 2: cbn; now rewrite map_length, fix_env_length.
+        
+        admit. + admit.
+        (*
+        cbn.
+        destruct (eqb_spec na0 na); subst.
+        -- rewrite add_recs''_not.
+           unfold Malfunction.Ident.Map.add.
+           unfold Malfunction.Ident.eqb.
+           subst Γn. subst. unfold Malfunction.Ident.Map.add. 
+           rewrite String.eqb_refl. reflexivity.
+           rewrite map_map. intros (? & ? & ?) % in_map_iff.
+           destruct x. destruct p. cbn in *. subst.
+           eapply Hfresh. revert Eqn H H0.
+           clear.
+           induction mfix in l |- *; destruct l; cbn; intros; try congruence.
+           inversion Eqn; subst; clear Eqn.
+           destruct p. destruct p. inversion H2; subst; clear H2.
+           destruct a. cbn in *.
+           destruct H0 as [[= -> -> ->] | ].
+           left. rewrite H in H4.
+           eapply (f_equal String.of_string) in H4. rewrite !of_string_to_string in H4. eauto.
+           right. eapply IHmfix; eauto.
+        -- epose proof (in_dec _ na0 (map fst mfix)) as [Hin | Hr].
+           ++ eapply in_map_iff in Hin as ([] & ? & Hin). cbn in *. subst.
+              eapply In_nth_error in Hin as [i Hi].
+              eapply All_Forall.Forall2_nth_error_Some_l in Hi as Hi'. destruct Hi' as (? & ? & ?). 2: exact Hl. cbn in *.
+              destruct x as [[]]. destruct H1; subst.
+              
+              destruct find eqn:Eq_find.
+              ** eapply find_some in Eq_find as [E1 E2]. destruct p. cbn in *.
+                 eapply eqb_eq in E2. subst.
+                 eassert (v = vRecClos mfix i Γ') as -> by admit. 
+                 cbn.
+                 erewrite add_recs''_spec.
+                 --- rewrite Hi. cbn. f_equal. f_equal. f_equal.
+                     2:{ 
+                      f_equal. f_equal. f_equal. f_equal. clear - Hl. induction Hl; cbn; try congruence.
+                      destruct y as [[]]. destruct H, x ; cbn in *; subst. f_equal. eapply IHHl.
+                     }
+                     cbn. unfold lookup.
+                     cbn. eapply funext. intros.
+                     { unfold Malfunction.Ident.Map.add.
+                       unfold Malfunction.Ident.eqb.
+                       destruct (String.eqb_spec x (String.to_string na)).
+                       +++ subst. rewrite of_string_to_string.                           
+                           change (String.eqb na na) with (eqb na na). rewrite eqb_refl. eauto.
+                       +++ change (String.eqb (String.of_string x) na) with (eqb (String.of_string x) na).
+                           destruct (eqb_spec (String.of_string x) na).
+                           *** subst. rewrite to_string_of_string in n1. congruence.
+                           *** reflexivity.
+                     }
+                     f_equal. f_equal. f_equal. f_equal. clear - Hl. induction Hl; cbn; try congruence.
+                     destruct y as [[]]. destruct H, x ; cbn in *; subst. f_equal. eapply IHHl.
+                 --- rewrite map_map. clear - Hnodup. induction l; cbn in *; inversion Hnodup; subst; econstructor.
+                     destruct a as [[]]; cbn in *. intros ([[]] & ? & ?) % in_map_iff. cbn in *. eapply H1.
+                     eapply in_map_iff. exists (t0, n0, t1). cbn. eauto. eapply (f_equal String.of_string) in H.
+                     rewrite !of_string_to_string in H. eauto. eauto.
+                 --- eapply in_map_iff. rewrite Hi. eexists (_, _, _). split. repeat f_equal. cbn. reflexivity.
+                     cbn. eapply nth_error_In; eauto.
+                 admit.
+              ** unshelve eapply find_none in Eq_find. refine (i0,  vRecClos mfix i (Γ')).
+                 cbn in *. rewrite eqb_refl in Eq_find. congruence.
+                 eapply nth_error_In.
+                 erewrite TemplateToPCUICCorrectness.nth_error_map2; eauto.
+                 now rewrite nth_error_map, Hi.
+                 todo "In_map2".
+           ++ todo "...".
+    + rewrite Mapply_spec. 2: congruence.
+      econstructor.
+      * cbn in IHHeval1. eapply IHHeval1; eauto.
+      * eauto.
+      * rewrite e0. set (Γn := (Malfunction.Ident.Map.add (fst (String.to_string (BasicAst.string_of_name (BasicAst.nNamed na)), fn)) (compile_value Σ av)
+       (fun x : Malfunction.Ident.t =>
+        match lookup (map (fun '(x0, v) => (x0, compile_value Σ v)) Γ') (String.of_string x) with
+        | Some v => v
+        | None => fail "notfound"
+        end))). 
+        unshelve econstructor. 3: econstructor.
+        3: eapply IHHeval2.
+        1: refine (add_recs'' Γn (map (fun '(x, y, t) => (bytestring.String.to_string (x), compile Σ (EAst.tLambda y t)) ) l)
+                     (map (fun '(x, y, t) => (bytestring.String.to_string (x), (bytestring.String.to_string (BasicAst.string_of_name y), compile Σ t) )) l)).
         1:{ unfold add_recs. rewrite <- Eqn.
             generalize ((map (fun x : string * EAst.term =>
              (String.to_string (fst x), compile Σ (snd x))) mfix)) at 1 3.
@@ -443,33 +617,19 @@ Proof.
             clear - Hl HΓ.
             induction Hl.
             * cbn. intros. f_equal.
-            * cbn. 
+            * cbn.
               destruct y as [[y1 y3] y2]. cbn in *. destruct x.
               cbn in *.
               destruct H as [-> ->]. cbn.
               simp compile. intros.
               erewrite IHHl. repeat f_equal.
         }
-        intros.
-        subst Γn. unfold Malfunction.Ident.Map.add.
-        rewrite lookup_add.
-        destruct (eqb_spec na (BasicAst.string_of_name na'_)). todo "sunny!".
-
-        all: admit.
-    + rewrite Mapply_spec. 2: congruence.
-      econstructor.
-      * cbn in IHHeval1. eapply IHHeval1; eauto.
-      * eauto.
-      * econstructor. 2: econstructor.
-        2: rewrite Hnth; cbn.
-        2: rewrite H4.
-        2: eapply IHHeval4.
-        all: admit.
+        todo "copy paste above". *)
   - (* fix *)
     cbn.
     destruct ((MCList.nth_error_Some' mfix (idx))) as [_ Hnth].
     forward Hnth.
-    assert (Datatypes.length mfix > 0) by lia.  1: lia. 
+    assert (Datatypes.length mfix > 0) by lia.  1: lia.
     assert ({ l | Forall2 (fun d '(x, y, b) => d.(EAst.dname) = BasicAst.nNamed x /\ d.(EAst.dbody) = EAst.tLambda y b) mfix l /\
                   NoDup (map (fun x => fst (fst x)) l) }) as [l [Hl Hnodup]].
     {
@@ -505,11 +665,13 @@ Proof.
         - destruct y as [[] ]. destruct H as [? ->].
           simp compile.
           repeat f_equal. 2: eapply IHHl.
-          now rewrite H. 
-      }   
+          now rewrite H.
+      }
     unshelve econstructor.
-    + refine (add_recs'' Γ_ (map (fun '(x, y, t) => (bytestring.String.to_string (x), compile Σ (EAst.tLambda y t)) ) l) 
+    + refine (add_recs'' Γ_ (map (fun '(x, y, t) => (bytestring.String.to_string (x), compile Σ (EAst.tLambda y t)) ) l)
                             (map (fun '(x, y, t) => (bytestring.String.to_string (x), (bytestring.String.to_string (BasicAst.string_of_name y), compile Σ t) )) l)).
+    + exact Γ_. 
+    + eapply equiv_wrt_refl.
     + rewrite MCList.map_InP_spec in *.
       unfold add_recs.
       rewrite <- Eqn.
@@ -520,7 +682,7 @@ Proof.
       clear - Hl. intros.
       induction Hl in Γ_.
       * cbn. reflexivity.
-      * cbn. 
+      * cbn.
         destruct y as [[y1 y3] y2]. cbn in *.
         destruct H as [? ->]. cbn.
         simp compile.
@@ -569,20 +731,31 @@ Proof.
     1: exact (compile Σ body).
     2:{ eapply IHHeval. reflexivity. }
     eapply in_flat_map.
-    unfold EGlobalEnv.declared_constant in *.    
+    unfold EGlobalEnv.declared_constant in *.
     eexists (_, _). split.
     + eapply lookup_env_In. cbn. eauto.
     + cbn. unfold compile_constant_decl. rewrite e. cbn. eauto.
   - (* constructor application *)
-    cbn. econstructor.
-    rewrite MCList.map_InP_spec.
-    clear l.
-    induction a.
-    + econstructor.
-    + econstructor.
-      * eapply IHa; eauto.
-      * eapply IHa0. destruct IHa. eapply a0.
-  - cbn. repeat econstructor.
+    cbn. destruct args; simp compile;
+    unfold lookup_constructor_args, EGlobalEnv.lookup_constructor in *;
+      destruct (EGlobalEnv.lookup_inductive) as [ [] | ]; cbn in *; try congruence.
+    + depelim a.
+      eapply eval_num. lia. 2: reflexivity.
+      todo "less constructors than Malfunction.Int63.wB".
+    + depelim a. cbn.
+      rewrite MCList.map_InP_spec.
+      clear l.
+      depelim IHa.
+      cbn. econstructor. econstructor. eapply e1; eauto. clear e1.
+      induction a.
+      * econstructor.
+      * cbn. econstructor.
+        -- eapply a0; eauto.
+        -- eapply IHa; eauto. eapply a0.
+  - cbn. unfold lookup_constructor_args, EGlobalEnv.lookup_constructor in *;
+      destruct (EGlobalEnv.lookup_inductive) as [ [] | ]; cbn in *; try congruence.
+    eapply eval_num. lia. 2:reflexivity.
+    todo "less constructors than Malfunction.Int63.wB".
   Unshelve. all:todo "evar".
-Admitted.
+Qed.
 Print Assumptions compile_correct.
